HW11

sf/Assignment11_10.v
@@ -6,21 +6,73 @@ Require Export Assignment11_09.
 **)
 
 Fixpoint tycheck (t: tm) (T: ty) : bool :=
-  FILL_IN_HERE.
+  match t with
+  | ttrue => 
+    match T with 
+    | TNat => false
+    | TBool => true
+    end
+  | tfalse =>
+    match T with 
+    | TNat => false
+    | TBool => true
+    end
+  | tif t1 t2 t3 =>
+      match (tycheck t1 TBool) with
+      | true => 
+        match (tycheck t2 T) && (tycheck t3 T) with
+        | true => true
+        | false => false
+        end
+      | false => false
+      end
+  | tzero =>
+    match T with
+    | TNat => true
+    | TBool => false
+    end
+  | tsucc t1 =>
+    match (tycheck t1 TNat) with
+    | true => 
+      match T with
+      | TNat => true
+      | TBool => false
+      end
+    | false => false
+    end
+  | tpred t1 =>
+    match (tycheck t1 TNat) with
+    | true => 
+      match T with
+      | TNat => true
+      | TBool => false
+      end
+    | false => false
+    end
+  | tiszero t1 =>
+    match (tycheck t1 TNat) with
+    | true => 
+      match T with
+      | TNat => false
+      | TBool => true
+      end
+    | false => false
+    end
+end.
 
 Example tycheck_ex1:
   tycheck
     (tif (tiszero (tpred (tsucc (tsucc tzero)))) ttrue (tiszero (tsucc tzero))) 
     TBool 
   = true.
-Proof. exact FILL_IN_HERE. Qed.
+Proof. compute. reflexivity. Qed.
 
 Example tycheck_ex2:
   tycheck
     (tif (tiszero (tpred (tsucc (tsucc tzero)))) tzero (tiszero (tsucc tzero))) 
     TBool 
   = false.
-Proof. exact FILL_IN_HERE. Qed.
+Proof. compute. reflexivity. Qed.
 
 (** Prove that the type checking function [tyeq: tm -> ty -> bool] is correct.
 
@@ -33,14 +85,88 @@ Theorem tycheck_correct1: forall t T
     (TYCHK: tycheck t T = true),
   |- t \in T.
 Proof.
-  exact FILL_IN_HERE.
+  induction t.
+  - destruct T.
+    + intros. eauto.
+    + intros. inversion TYCHK.
+  - destruct T.
+    + intros. eauto.
+    + intros. inversion TYCHK.
+  - destruct T.
+    + intros. constructor. 
+      * inversion TYCHK. apply IHt1. destruct (tycheck t1 TBool) eqn: H.
+        reflexivity. inversion H0.
+      * inversion TYCHK. destruct (tycheck t1 TBool) eqn: H.
+        { destruct (tycheck t2 TBool && tycheck t3 TBool) eqn: H1.
+          apply andb_prop in H1. inversion H1. apply IHt2. assumption.
+          inversion H0.
+        } inversion H0.
+      * inversion TYCHK. destruct (tycheck t1 TBool) eqn: H.
+        { destruct (tycheck t2 TBool && tycheck t3 TBool) eqn: H1.
+          apply andb_prop in H1. inversion H1. apply IHt3. assumption.
+          inversion H0.
+        } inversion H0.
+    + intros. constructor.
+      * inversion TYCHK. apply IHt1. destruct (tycheck t1 TBool) eqn: H.
+        reflexivity. inversion H0.
+      * inversion TYCHK. destruct (tycheck t1 TBool) eqn: H.
+        { destruct (tycheck t2 TNat && tycheck t3 TNat) eqn: H1.
+          apply andb_prop in H1. inversion H1. apply IHt2. assumption.
+          inversion H0.
+        } inversion H0.
+      * inversion TYCHK. destruct (tycheck t1 TBool) eqn: H.
+        { destruct (tycheck t2 TNat && tycheck t3 TNat) eqn: H1.
+          apply andb_prop in H1. inversion H1. apply IHt3. assumption.
+          inversion H0.
+        } inversion H0.
+  - destruct T.
+    + intros. inversion TYCHK.
+    + intros. eauto.
+  - destruct T.
+    + intros. inversion TYCHK. destruct (tycheck t TNat) eqn: H; inversion H0.
+    + intros. inversion TYCHK ; subst.  destruct (tycheck t TNat) eqn: H.
+      * apply IHt in H. eauto.
+      * inversion H0.
+  - destruct T.
+    + intros. inversion TYCHK. destruct (tycheck t TNat) eqn: H; inversion H0.
+    + intros. inversion TYCHK ; subst.  destruct (tycheck t TNat) eqn: H.
+      * apply IHt in H. eauto.
+      * inversion H0.
+  - destruct T.
+    + intros. inversion TYCHK ; subst. destruct (tycheck t TNat) eqn: H.
+      * apply IHt in H. constructor. eauto.
+      * inversion H0.
+    + intros. inversion TYCHK ; subst. destruct (tycheck t TNat) eqn: H ; inversion H0.
 Qed.
 
 Theorem tycheck_correct2: forall t T
     (HASTY: |- t \in T),
   tycheck t T = true.
 Proof.
-  exact FILL_IN_HERE.
+  induction t.
+  - destruct T.
+    + intros. eauto.
+    + intros. inversion HASTY.
+  - destruct T.
+    + intros. eauto.
+    + intros. inversion HASTY.
+  - destruct T.
+    + intros. inversion HASTY ; subst. apply IHt1 in H2. apply IHt2 in H4.
+      apply IHt3 in H5. simpl. rewrite H2. rewrite H4. rewrite H5. reflexivity.
+    + intros. inversion HASTY ; subst. apply IHt1 in H2. apply IHt2 in H4.
+      apply IHt3 in H5. simpl. rewrite H2. rewrite H4. rewrite H5. reflexivity. 
+  - destruct T.
+    + intros. inversion HASTY.
+    + intros. eauto.
+  - destruct T.
+    + intros. inversion HASTY.
+    + intros. inversion HASTY ; subst. simpl. apply IHt in H0. rewrite H0. reflexivity.
+  - destruct T.
+    + intros. inversion HASTY.
+    + intros. inversion HASTY ; subst. simpl. apply IHt in H0. rewrite H0. reflexivity.
+  - destruct T.
+    + intros. inversion HASTY ; subst. apply IHt in H0. simpl. rewrite H0. reflexivity.
+    + intros. inversion HASTY.
 Qed.
 
 (*-- Check --*)
