sf/Assignment11_03.v
@@ -9,10 +9,36 @@ Require Export Assignment11_02.
 Theorem step_deterministic:
   deterministic step.
 Proof with eauto.
-  exact FILL_IN_HERE.
+  unfold deterministic. intros. generalize dependent y2.
+  induction H ; intros.
+  - inversion H0; subst. reflexivity. inversion H4.
+  - inversion H0; subst. reflexivity. inversion H4.
+  - inversion H0; subst.
+    + inversion H.
+    + inversion H.
+    + apply IHstep in H5. subst. reflexivity.
+  - inversion H0 ; subst. apply IHstep in H2. subst. reflexivity.
+  - inversion H0. reflexivity. solve by inversion.
+  - inversion H0 ; subst. reflexivity. assert (value t1). eauto. inversion H2 ; subst.
+    apply value_is_nf in H1. unfold normal_form in H1. unfold not in H1. 
+    assert (exists t':tm, t1 ==> t'). eauto. apply H1 in H3. inversion H3.
+  - inversion H0; subst. 
+    + solve by inversion.
+    + inversion H ; subst. assert (value y2). eauto. apply value_is_nf in H1. unfold normal_form in H1.
+      assert (exists t':tm, y2 ==> t'). eauto. apply H1 in H4. inversion H4.
+    + inversion H0 ; subst. inversion H3. apply IHstep in H2. subst. reflexivity.
+  - inversion H0. reflexivity. inversion H1.
+  - inversion H0; subst. reflexivity. inversion H2 ; subst. 
+    assert (value t1). eauto. apply value_is_nf in H1. unfold normal_form in H1.
+    assert (exists t':tm, t1 ==> t'). eauto. apply H1 in H4. inversion H4.
+  - inversion H0; subst.
+    + inversion H.
+    + inversion H ; subst.  
+      assert (value t0). eauto. apply value_is_nf in H1. unfold normal_form in H1.
+      assert (exists t':tm, t0 ==> t'). eauto. apply H1 in H4. inversion H4.
+    + apply IHstep in H2. subst. reflexivity.
 Qed.
 
 (*-- Check --*)
 Check step_deterministic:
   deterministic step.
-
